Some cleanup and syncing with paper

theories/Stlc/Unification.v
@@ -58,9 +58,19 @@ Ltac folddefs :=
     match goal with
     | |- context[@Tri.refl ?w] =>
         change_no_check (@Tri.refl w) with (@refl Tri _ w)
+    | |- context[Tri.cons ?x ?t refl] =>
+        change_no_check (Tri.cons x t refl) with (thick x t)
     | |- context[Tri.cons ?x ?t ?r] =>
         change_no_check (Tri.cons x t r) with (thick x t ⊙⁻ r)
     end.
+
+Definition löb {A} : (⊢ʷ ▷A -> A) -> (⊢ʷ A) :=
+  fun step w => ctx.remove_acc_rect A step (ctx.remove_acc_all w).
+
+Definition löb_elim {A} (step : ⊢ʷ ▷A -> A) (P : forall w, A w -> Prop)
+  (IH: forall w (f : ▷A w) (pf : forall x xIn, P (w - x) (f x xIn)), P w (step w f)) :
+  forall w, P w (löb step w).
+Proof. intros w. unfold löb. induction (ctx.remove_acc_all w). now apply IH. Qed.
 
 Section Operations.
 
@@ -140,7 +150,7 @@ Section Implementation.
   Definition ctrue : ⊢ʷ C :=
     fun w0 w1 r01 => pure tt.
   Definition cfalse : ⊢ʷ C :=
-    fun w0 w1 r01 => None.
+    fun w0 w1 r01 => fail.
   Definition cand : ⊢ʷ C -> C -> C :=
     fun w0 c1 c2 w1 r01 =>
       bind (c1 w1 r01) (fun w2 r12 _ => _4 c2 r01 r12).
@@ -150,82 +160,81 @@ Section Implementation.
   Definition BoxUnifier : TYPE :=
     Ṫy -> Ṫy -> C.
 
-  Definition flex : ⊢ʷ Ṫy -> ∀ α, ctx.In α -> OptionDiamond Unit :=
-    fun w t α αIn =>
-      match varview t with
+  Definition flex : ⊢ʷ ∀ α, ctx.In α -> Ṫy -> OptionDiamond Unit :=
+    fun w α αIn τ =>
+      match varview τ with
       | is_var βIn =>
           match ctx.occurs_check_view αIn βIn with
           | ctx.Same _      => pure tt
           | ctx.Diff _ βIn' => singleton αIn (ṫy.var βIn')
           end
       | not_var _ =>
-          match occurs_check t αIn with
-          | Some t' => singleton αIn t'
+          match occurs_check τ αIn with
+          | Some τ' => singleton αIn τ'
           | None    => fail
           end
       end.
+  #[global] Arguments flex {w} α {αIn} τ : rename.
 
   Section MguO.
 
-    Context [w] (lmgu : ▷BoxUnifier w).
+    Context [w] (lamgu : ▷BoxUnifier w).
+    Arguments lamgu {_ _} _ _ {_} _.
 
-    Definition boxflex (t : Ṫy w) {x} (xIn : x ∈ w) : C w :=
-      Tri.box_intro_split
-        (flex t xIn)
-        (fun z zIn u =>
-           let ζ := thick (Θ := Tri) z u in
-           lmgu _ (lk ζ xIn) (persist t ζ)).
+    Definition aflex α {αIn : α ∈ w} (τ : Ṫy w) : C w :=
+      fun _ θ =>
+        match θ with
+        | Tri.refl         => flex α τ
+        | Tri.cons β τ' θ' => lamgu (lk (thick β τ') αIn) τ[thick β τ'] θ'
+        end.
+    #[global] Arguments aflex α {αIn} τ [w1] _.
 
-    Definition boxmgu : BoxUnifier w :=
+    Definition atrav : (Ṫy -> Ṫy -> C)%W w :=
       fix bmgu s t {struct s} :=
         match s , t with
-        | ṫy.var xIn    , t             => boxflex t xIn
-        | s             , ṫy.var yIn    => boxflex s yIn
+        | @ṫy.var _ α _  , t             => aflex α t
+        | s             , @ṫy.var _ β _  => aflex β s
         | ṫy.bool       , ṫy.bool       => ctrue
         | ṫy.func s1 s2 , ṫy.func t1 t2 => cand (bmgu s1 t1) (bmgu s2 t2)
         | _             , _             => cfalse
         end.
 
-    Section boxmgu_elim.
+    Section atrav_elim.
 
       Context (P : Ṫy w -> Ṫy w -> C w -> Type).
-      Context (fflex1 : forall (x : nat) (xIn : x ∈ w) (t : Ṫy w), P (ṫy.var xIn) t (boxflex t xIn)).
-      Context (fflex2 : forall (x : nat) (xIn : x ∈ w) (t : Ṫy w), P t (ṫy.var xIn) (boxflex t xIn)).
+      Context (fflex1 : forall (x : nat) (xIn : x ∈ w) (t : Ṫy w), P (ṫy.var xIn) t (aflex x t)).
+      Context (fflex2 : forall (x : nat) (xIn : x ∈ w) (t : Ṫy w), P t (ṫy.var xIn) (aflex x t)).
       Context (fbool : P ṫy.bool ṫy.bool ctrue).
       Context (fbool_func : forall T1 T2 : Ṫy w, P ṫy.bool (ṫy.func T1 T2) cfalse).
       Context (ffunc_bool : forall T1 T2 : Ṫy w, P (ṫy.func T1 T2) ṫy.bool cfalse).
       Context (ffunc : forall s1 s2 t1 t2 : Ṫy w,
-        (P s1 t1 (boxmgu s1 t1)) ->
-        (P s2 t2 (boxmgu s2 t2)) ->
+        (P s1 t1 (atrav s1 t1)) ->
+        (P s2 t2 (atrav s2 t2)) ->
         P (ṫy.func s1 s2) (ṫy.func t1 t2)
-          (cand (boxmgu s1 t1) (boxmgu s2 t2))).
+          (cand (atrav s1 t1) (atrav s2 t2))).
 
-      Lemma boxmgu_elim : forall (t1 t2 : Ṫy w), P t1 t2 (boxmgu t1 t2).
+      Lemma atrav_elim : forall (t1 t2 : Ṫy w), P t1 t2 (atrav t1 t2).
       Proof. induction t1; intros t2; cbn; auto; destruct t2; auto. Qed.
 
-    End boxmgu_elim.
+    End atrav_elim.
 
   End MguO.
 
-  Definition bmgu_aux : ⊢ʷ ctx.remove_acc -> BoxUnifier :=
-    fix bmgu {w} d {struct d} : BoxUnifier w :=
-      boxmgu (fun α αIn => bmgu (ctx.remove_acc_inv d αIn)).
-
-  Definition bmgu : ⊢ʷ BoxUnifier :=
-    fun w => bmgu_aux (ctx.remove_acc_all w).
+  Definition amgu : ⊢ʷ BoxUnifier :=
+    löb atrav.
 
   Definition mgu : ⊢ʷ Ṫy -> Ṫy -> OptionDiamond Unit :=
-    fun w s t => T (@bmgu w s t).
+    fun w s t => T (@amgu w s t).
 
-  Definition boxsolvelist : ⊢ʷ List (Prod Ṫy Ṫy) -> C :=
-    fix solve {w} cs {struct cs} :=
+  Definition asolver : ⊢ʷ List (Prod Ṫy Ṫy) -> C :=
+    fix asolver {w} cs {struct cs} :=
       match cs with
       | List.nil             => ctrue
-      | List.cons (t1,t2) cs => cand (bmgu t1 t2) (solve cs)
+      | List.cons (t1,t2) cs => cand (amgu t1 t2) (asolver cs)
       end.
 
-  Definition solvelist : ⊢ʷ List (Prod Ṫy Ṫy) -> OptionDiamond Unit :=
-    fun w cs => boxsolvelist cs refl.
+  Definition solver : ⊢ʷ List (Prod Ṫy Ṫy) -> OptionDiamond Unit :=
+    fun w cs => asolver cs refl.
 
   Import option.notations.
 
@@ -233,7 +242,7 @@ Section Implementation.
     Diamond alloc.acc_alloc (List (Ṫy * Ṫy) * A) ctx.nil ->
     Option (Diamond alloc.acc_alloc A) ctx.nil :=
     fun '(existT w1 (θ1, (cs, a))) =>
-      '(existT w2 (θ2, tt))      <- solvelist cs;;
+      '(existT w2 (θ2, tt))      <- solver cs;;
       Some (existT w2 (alloc.nil_l,persist a θ2)).
 
   Definition optiondiamond2schematic {A} :
@@ -271,7 +280,7 @@ Section Correctness.
         instpred (bu t1 t2 w1 θ1) ⊣⊢ₚ (t1 =ₚ t2)[θ1].
 
   Lemma flex_correct {w α} (αIn : α ∈ w) (t : Ṫy w) :
-    instpred (flex t αIn) ⊣⊢ₚ ṫy.var αIn =ₚ t.
+    instpred (flex α t) ⊣⊢ₚ ṫy.var αIn =ₚ t.
   Proof.
     unfold flex. destruct varview; cbn.
     - destruct ctx.occurs_check_view; cbn.
@@ -286,23 +295,23 @@ Section Correctness.
 
   Section InnerRecursion.
 
-    Context [w] (lmgu : ▷BoxUnifier w).
-    Context (lmgu_correct : forall x (xIn : x ∈ w),
-                BoxUnifierCorrect (lmgu xIn)).
+    Context [w] (lamgu : ▷BoxUnifier w).
+    Context (lamgu_correct : forall x (xIn : x ∈ w),
+                BoxUnifierCorrect (lamgu xIn)).
 
-    Lemma boxflex_correct {α} (αIn : α ∈ w) (t : Ṫy w) w1 (θ1 : w ⊒⁻ w1) :
-      instpred (boxflex lmgu t αIn θ1) ⊣⊢ₚ (ṫy.var αIn =ₚ t)[θ1].
+    Lemma aflex_correct {α} (αIn : α ∈ w) (t : Ṫy w) w1 (θ1 : w ⊒⁻ w1) :
+      instpred (aflex lamgu α t θ1) ⊣⊢ₚ (ṫy.var αIn =ₚ t)[θ1].
     Proof.
       destruct θ1; cbn; folddefs.
       - now rewrite flex_correct, persist_pred_refl.
-      - now rewrite lmgu_correct, !persist_eq, !persist_trans.
+      - now rewrite lamgu_correct, !persist_eq, !persist_trans.
     Qed.
 
-    Lemma boxmgu_correct : BoxUnifierCorrect (boxmgu lmgu).
+    Lemma atrav_correct : BoxUnifierCorrect (atrav lamgu).
     Proof.
-      intros t1 t2. pattern (boxmgu lmgu t1 t2). apply boxmgu_elim; clear t1 t2.
-      - intros α αIn t w1 θ1. now rewrite boxflex_correct.
-      - intros α αIn t w1 θ1. now rewrite boxflex_correct.
+      intros t1 t2. pattern (atrav lamgu t1 t2). apply atrav_elim; clear t1 t2.
+      - intros α αIn t w1 θ1. now rewrite aflex_correct.
+      - intros α αIn t w1 θ1. now rewrite aflex_correct.
       - intros. now rewrite instpred_ctrue, eqₚ_refl.
       - intros. now rewrite instpred_cfalse, peq_ty_noconfusion.
       - intros. now rewrite instpred_cfalse, peq_ty_noconfusion.
@@ -312,60 +321,26 @@ Section Correctness.
 
   End InnerRecursion.
 
-  Section OuterRecursion.
-
-    Lemma bmgu_aux_correct w d : BoxUnifierCorrect (@bmgu_aux w d).
-    Proof. induction d. cbn. now apply boxmgu_correct. Qed.
-
-    Lemma bmgu_correct w : BoxUnifierCorrect (@bmgu w).
-    Proof. apply bmgu_aux_correct. Qed.
-
-  End OuterRecursion.
+  Lemma amgu_correct : forall w, BoxUnifierCorrect (@amgu w).
+  Proof. apply löb_elim, atrav_correct. Qed.
 
   Definition mgu_correct w (t1 t2 : Ṫy w) :
     instpred (mgu t1 t2) ⊣⊢ₚ t1 =ₚ t2.
-  Proof. unfold mgu, T. now rewrite bmgu_correct, persist_pred_refl. Qed.
+  Proof. unfold mgu, T. now rewrite amgu_correct, persist_pred_refl. Qed.
 
   #[local] Existing Instance instpred_prod_ty.
 
-  Lemma boxsolvelist_correct {w0} (C : List (Ṫy * Ṫy) w0) :
+  Lemma asolver_correct {w0} (C : List (Ṫy * Ṫy) w0) :
     forall w1 (θ1 : w0 ⊒⁻ w1),
-      instpred (boxsolvelist C θ1) ⊣⊢ₚ (instpred C)[θ1].
+      instpred (asolver C θ1) ⊣⊢ₚ (instpred C)[θ1].
   Proof.
     induction C as [|[t1 t2]]; cbn - [ctrue cand]; intros.
     - now rewrite instpred_ctrue.
-    - apply instpred_cand_intro; auto. intros. apply bmgu_correct.
+    - apply instpred_cand_intro; auto. intros. apply amgu_correct.
   Qed.
 
-  Lemma solvelist_correct {w} (C : List (Ṫy * Ṫy) w) :
-    instpred (solvelist C) ⊣⊢ₚ instpred C.
-  Proof.
-    unfold solvelist, T.
-    now rewrite boxsolvelist_correct, persist_pred_refl.
-  Qed.
+  Lemma solver_correct {w} (C : List (Ṫy * Ṫy) w) :
+    instpred (solver C) ⊣⊢ₚ instpred C.
+  Proof. unfold solver, T. now rewrite asolver_correct, persist_pred_refl. Qed.
 
 End Correctness.
-
-Module Löb.
-
-  Section Recursor.
-
-    Context (A : TYPE) (step : ⊢ʷ ▷A -> A).
-
-    #[local] Obligation Tactic := auto using Nat.eq_le_incl, ctx.length_remove.
-    Equations Löb {w : World} : A w by wf (ctx.length w) :=
-    Löb := step (fun _ _ => Löb).
-    #[global] Arguments Löb : clear implicits.
-
-  End Recursor.
-
-  Definition bmgu : ⊢ʷ BoxUnifier :=
-    fun w s t => Löb boxmgu _ s t.
-
-  Lemma bmgu_correct w : BoxUnifierCorrect (@bmgu w).
-  Proof.
-    pattern (@bmgu w). revert w. apply Löb_elim.
-    intros w IH. now apply boxmgu_correct.
-  Qed.
-
-End Löb.
