theories/Stlc/Symbolic/FreeReconstruct.v
@@ -353,9 +353,9 @@ Section Correctness.
     apply proper_wp_option_bientails.
     intros (w & θ & C & [t' ee']). cbn.
     rewrite wp_optiondiamond_bind'.
-    rewrite <- solvelist_correct.
+    rewrite <- solver_correct.
     unfold wp_optiondiamond.
-    destruct (solvelist C) as [(w2 & θ2 & [])|]; cbn.
+    destruct (solver C) as [(w2 & θ2 & [])|]; cbn.
     - rewrite Acc.and_wp_l. wsimpl. clear.
       rewrite eqₚ_sym.
       generalize (t' =ₚ lift t w2). clear. intros P.
@@ -385,7 +385,5 @@ Section Correctness.
     destruct reconstruct_optiondiamond as [(w & θ & [t' ee'])|]; cbn; auto.
     apply base.exist_proper. intros ι. pred_unfold. intuition.
   Qed.
-
-  Print Assumptions correctness.
 
 End Correctness.
